TestModels/CallingAWSSDKFromLocalService/test/WrappedSimpleCallingAWSSDKFromLocalServiceTest.dfy
@@ -5,6 +5,7 @@ include "SimpleCallingAWSSDKFromLocalServiceImplTest.dfy"
 
 module WrappedSimpleCallingAWSSDKFromLocalServiceTest {
   import Com.Amazonaws.Kms
+  import DDB = Com.Amazonaws.Dynamodb
   import SimpleCallingAWSSDKFromLocalService
 
   import opened WrappedSimpleCallingAWSSDKFromLocalServiceService
@@ -13,9 +14,16 @@ module WrappedSimpleCallingAWSSDKFromLocalServiceTest {
   import opened StandardLibrary.UInt
   import opened SimpleCallingawssdkfromlocalserviceTypes
 
+  const TABLE_ARN_FAILURE_CASE := "arn:aws:dynamodb:us-west-2:370957321024:table/TestTableFailure"
   const NONEXISTENT_KEY_ID := "arn:aws:kms:us-west-2:658956600833:key/b3537ef1-d8dc-4780-9f5a-55776cbb2f7g"
   // The string "asdf" as bytes
   const PLAIN_TEXT: Kms.Types.PlaintextType := [ 97, 115, 100, 102 ]
+
+  method{:test} TestCallDDBScan() {
+    var client :- expect WrappedSimpleCallingAWSSDKFromLocalServiceService.WrappedSimpleCallingAWSSDKFromLocalService();
+    SimpleCallingAWSSDKFromLocalServiceImplTest.TestCallDDBScan_Success(client);
+    TestCallDDBScan_Failure(client);
+  }
 
   method{:test} TestCallKMSEncrypt() {
     var client :- expect WrappedSimpleCallingAWSSDKFromLocalServiceService.WrappedSimpleCallingAWSSDKFromLocalService();
@@ -41,5 +49,16 @@ module WrappedSimpleCallingAWSSDKFromLocalServiceTest {
     var resFailure_NonExistent := client.CallKMSEncrypt(SimpleCallingAWSSDKFromLocalService.Types.CallKMSEncryptInput(kmsClient := kmsClient, keyId := NONEXISTENT_KEY_ID, plaintext := PLAIN_TEXT));
     expect resFailure_NonExistent.Failure?;
     expect resFailure_NonExistent.error.ComAmazonawsKms.NotFoundException?;
+  }
+
+  method TestCallDDBScan_Failure(client: ISimpleCallingAWSSDKFromLocalServiceClient)
+    requires client.ValidState()
+    modifies client.Modifies
+    ensures client.ValidState()
+  {
+    var ddbClient :- expect DDB.DynamoDBClient();
+    var resFailure := client.CallDDBGetItem(SimpleCallingAWSSDKFromLocalService.Types.CallDDBGetItemInput(ddbClient := ddbClient, tableArn := TABLE_ARN_FAILURE_CASE));
+    print(resFailure);
+    expect resFailure.Failure?;
   }
 }
